Getopt/Options: some cleanup
'Help' was never returned by Getopt.

src/basic/FStarC.Options.fst
@@ -227,6 +227,7 @@ let defaults =
       ("extract_module"               , List []);
       ("extract_namespace"            , List []);
       ("full_context_dependency"      , Bool true);
+      ("help"                         , Bool false);
       ("hide_uvar_nums"               , Bool false);
       ("hint_hook"                    , Unset);
       ("hint_info"                    , Bool false);
@@ -494,6 +495,7 @@ let get_extract                 ()      = lookup_opt "extract"                  
 let get_extract_module          ()      = lookup_opt "extract_module"           (as_list as_string)
 let get_extract_namespace       ()      = lookup_opt "extract_namespace"        (as_list as_string)
 let get_force                   ()      = lookup_opt "force"                    as_bool
+let get_help                    ()      = lookup_opt "help"                     as_bool
 let get_hide_uvar_nums          ()      = lookup_opt "hide_uvar_nums"           as_bool
 let get_hint_info               ()      = lookup_opt "hint_info"                as_bool
 let get_hint_dir                ()      = lookup_opt "hint_dir"                 (as_option as_string)
@@ -1661,9 +1663,7 @@ let rec specs_with_types warn_unsafe : list (char & string & opt_type & Pprint.d
           This option is a module or namespace selector, like many other options (e.g., `--extract`)");
 
   ( 'h',
-    "help",
-     WithSideEffect ((fun _ -> display_usage_aux (specs warn_unsafe); exit 0),
-                     (Const (Bool true))),
+    "help", Const (Bool true),
     text "Display this information");
 
   ( noshort,
@@ -2074,6 +2074,7 @@ let message_format               () =
 
 let force                        () = get_force ()
 let full_context_dependency      () = true
+let help                         () = get_help                        ()
 let hide_uvar_nums               () = get_hide_uvar_nums              ()
 let hint_info                    () = get_hint_info                   ()
                                     || get_query_stats                ()
