src/basic/FStarC.Getopt.fsti
@@ -28,7 +28,6 @@ type opt = opt' unit
 
 type parse_cmdline_res =
   | Empty
-  | Help
   | Error of (string & string) // second arg is the long name of the failed option
   | Success
 
